Sorting the events in SubToFullExec

src/SubToFullExec.v
@@ -793,9 +793,17 @@ Proof using.
   eapply dom_rel_mori; eauto; basic_solver.
 Qed.
 
-Lemma sub_to_full_exec_sort G G' cmt l (ord : relation thread_id)
+Definition lord : relation location := fun x y => True.
+
+Lemma lord_strict_total : strict_total_order ⊤₁ lord.
+Proof using.
+  admit.
+Admitted.
+
+Lemma sub_to_full_exec_sort G G' cmt l
+    (ord : relation thread_id)
     (ORD : strict_total_order ⊤₁ ord)
-    (ORB : tid ↓ ord ⊆ sb G')
+    (ORB : min_elt ord tid_init)
     (ORDRF : restr_rel (acts_set G' \₁ acts_set G)
               (rf G' ⨾ ⦗acts_set G' \₁ cmt⦘) ⊆ tid ↓ ord)
     (ENUM : SubToFullExecInternal.enumd_diff G G' cmt l) :
@@ -803,12 +811,74 @@ Lemma sub_to_full_exec_sort G G' cmt l (ord : relation thread_id)
       G
       G'
       cmt
-      (isort (tid ↓ ord ∪ sb G') l).
+      (isort (InitEvent ↑ lord ∪ tid ↓ ord ∪ ext_sb) l).
 Proof using.
   (* Setup *)
-  set (sord := tid ↓ ord ∪ sb G').
+  assert (LORD : strict_total_order ⊤₁ lord).
+  { apply lord_strict_total. }
+  desf.
+  set (sord := InitEvent ↑ lord ∪ tid ↓ ord ∪ ext_sb).
+  assert (OTOTAL : is_total ⊤₁ ord).
+  { apply ORD. }
+  assert (LOTOTAL : is_total ⊤₁ lord).
+  { apply LORD. }
+  assert (OTRANS : transitive ord).
+  { apply ORD. }
+  assert (LOTRANS : transitive lord).
+  { apply LORD. }
+  assert (IRR : irreflexive sord).
+  { subst sord. unfolder. intros x HREL. desf.
+    { eapply LORD. eauto. }
+    { eapply ORD. eauto. }
+    eapply ext_sb_irr. eauto. }
   assert (TOTAL : strict_total_order ⊤₁ sord).
-  { admit. }
+  { subst sord. constructor; ins.
+    { constructor; ins.
+      unfolder. intros x y z R1 R2. desf; ins.
+      { do 2 left. do 2 eexists; splits.
+        { eapply LOTRANS with (y := y'0); eauto. }
+        all: ins. }
+      { exfalso. eapply ORB; eauto. }
+      { destruct x; ins. }
+      { destruct z as [zl | zt zn]; eauto. }
+      { left. right. splits; ins.
+        eapply OTRANS; eauto. }
+      { apply ext_sb_tid_init in R1. desf.
+        { left. right. now rewrite R1. }
+        destruct (classic (is_init y)) as [YINIT|NINT].
+        { destruct x as [xl | xt xn],
+                   y as [yl | yt yn],
+                   z as [zl | zt zn]; ins.
+          all: eauto 11. }
+        right.
+        destruct x as [xl | xt xn],
+                 z as [zl | zt zn]; ins.
+        eapply ORB; eauto. }
+      { desf. eauto. }
+      { apply ext_sb_tid_init in R2. desf.
+        { left. right. now rewrite <- R2. }
+        destruct (classic (is_init x)) as [XINIT|NINT].
+        { destruct x as [xl | xt xn],
+                   y as [yl | yt yn]; ins.
+          exfalso. eapply ORD; eauto. }
+        destruct x as [xl | xt xn],
+                 y as [yl | yt yn]; ins.
+        exfalso. eapply ORB; eauto. }
+      right. now apply ext_sb_trans with (y := y). }
+    unfolder. intros x _ y _ ACTNEQ.
+    destruct (classic (is_init x)) as [XINIT|XNIT],
+             (classic (is_init y)) as [YINIT|YNIT].
+    all: destruct x as [xl | xt xn],
+                  y as [yl | yt yn]; ins.
+    all: eauto.
+    { destruct LOTOTAL with xl yl; ins.
+      all: eauto 11.
+      congruence. }
+    destruct (classic (xt = yt)) as [TEQ|TNEQ]; subst.
+    { destruct NPeano.Nat.lt_total with xn yn as [LT | [EQ | GT]].
+      all: eauto 11.
+      congruence. }
+    destruct OTOTAL with xt yt; eauto; ins. }
   assert (DIFF : acts_set G' \₁ acts_set G ≡₁
             (fun x => In x (isort sord l))).
   { rewrite (SubToFullExecInternal.diff_elems ENUM).
@@ -817,29 +887,27 @@ Proof using.
   (* Proof *)
   constructor; ins.
   { apply NoDup_StronglySorted with (r := sord).
-    { subst sord. unfolder. intros x HREL. desf.
-      { eapply ORD. eauto. }
-      eapply sb_irr. eauto. }
-    apply StronglySorted_isort; ins.
-    apply ENUM. }
+    { ins. }
+    apply StronglySorted_isort, ENUM; ins. }
   { intros x y (SB & DOM & CODOM).
     apply DIFF in DOM, CODOM.
     apply total_order_from_isort; ins.
     { apply ENUM. }
     unfolder; splits.
     all: try now eapply in_isort_iff; eauto.
-    subst sord. now right. }
+    subst sord. red in SB. unfolder in SB. desf.
+    now right. }
   { intros x y (y' & (RF & DOM & CODOM) & EQ & NCMT).
     subst y'. apply DIFF in DOM, CODOM.
     apply total_order_from_isort; ins.
     { apply ENUM. }
     unfolder; splits.
     all: try now eapply in_isort_iff; eauto.
-    subst sord. left. apply ORDRF.
+    subst sord. left. right. apply ORDRF.
     apply DIFF in DOM, CODOM.
     split; eauto.
     exists y; unfolder; eauto. }
   apply ENUM.
-Admitted.
+Qed.
 
 End SubToFullExec.
